Move to simple assembly language

Rules.thy
@@ -1,5 +1,5 @@
 theory Rules
-  imports Interference Syntactic_Refine
+  imports Interference
 begin
 
 chapter \<open>Rules\<close>
@@ -19,22 +19,15 @@ inductive rules :: "'b rpred \<Rightarrow> 'b rpred \<Rightarrow> 'b set \<Right
   where
   basic[intro]:  "R,G \<turnstile>\<^sub>A P {\<alpha>} Q \<Longrightarrow> R,G \<turnstile> P { Basic \<alpha> } Q" |
   nil[intro]:    "stable R P \<Longrightarrow> R,G \<turnstile> P { Nil } P" |
-  seq[intro]:    "R,G \<turnstile> Q { c\<^sub>2 } M \<Longrightarrow> R,G \<turnstile> P { c\<^sub>1 } Q \<Longrightarrow> R,G \<turnstile> P { c\<^sub>1 ;; c\<^sub>2 } M" |
-  ord[intro]:    "R,G \<turnstile> Q { c\<^sub>2 } M \<Longrightarrow> R,G \<turnstile> P { c\<^sub>1 } Q \<Longrightarrow> R,G \<turnstile> P { c\<^sub>1 \<cdot> c\<^sub>2 } M" |
+  seq[intro]:    "R,G \<turnstile> Q { c\<^sub>2 } M \<Longrightarrow> R,G \<turnstile> P { c\<^sub>1 } Q \<Longrightarrow> R,G \<turnstile> P { c\<^sub>1 ; c\<^sub>2 } M" |
   choice[intro]: "R,G \<turnstile> P { c\<^sub>1 } Q \<Longrightarrow> R,G \<turnstile> P { c\<^sub>2 } Q \<Longrightarrow> R,G \<turnstile> P { c\<^sub>1 \<sqinter> c\<^sub>2 } Q" |
-  seqset[intro]: "\<forall>s \<in> S. R,G \<turnstile> P { seq2com s } Q \<Longrightarrow> R,G \<turnstile> P { \<Sqinter> S } Q" |
   loop[intro]:   "stable R P \<Longrightarrow> R,G \<turnstile> P { c } P \<Longrightarrow> R,G \<turnstile> P { c* } P" |
-  state[intro]:  "R,G \<turnstile> P { c } Q \<Longrightarrow> inter R G c \<Longrightarrow> 
-                  thr\<^sub>R op R,thr\<^sub>G op G \<turnstile> thr\<^sub>P op l P { State l op c } thr\<^sub>Q op Q" |
-  thread[intro]: "R,G \<turnstile> P { c } Q \<Longrightarrow> inter R G c \<Longrightarrow> 
-                  thr\<^sub>R op R,thr\<^sub>G op G \<turnstile> thr\<^sub>A op P { Thread op c } thr\<^sub>Q op Q" |
+  thread[intro]: "R,G \<turnstile> P { c } Q \<Longrightarrow> inter R G c \<Longrightarrow> R,G \<turnstile> P { Thread c } Q" |
   par[intro]:    "R\<^sub>1,G\<^sub>1 \<turnstile> P\<^sub>1 { c\<^sub>1 } Q\<^sub>1 \<Longrightarrow> R\<^sub>2,G\<^sub>2 \<turnstile> P\<^sub>2 { c\<^sub>2 } Q\<^sub>2 \<Longrightarrow> G\<^sub>2 \<subseteq> R\<^sub>1 \<Longrightarrow> G\<^sub>1 \<subseteq> R\<^sub>2 \<Longrightarrow> 
                   R\<^sub>1 \<inter> R\<^sub>2,G\<^sub>1 \<union> G\<^sub>2 \<turnstile> P\<^sub>1 \<inter> P\<^sub>2 { c\<^sub>1 || c\<^sub>2 } (Q\<^sub>1 \<inter> Q\<^sub>2)" |
   conseq[intro]: "R,G \<turnstile> P { c } Q \<Longrightarrow> P' \<subseteq> P \<Longrightarrow> R' \<subseteq> R \<Longrightarrow> G \<subseteq> G' \<Longrightarrow> Q \<subseteq> Q' \<Longrightarrow> 
-                  R',G' \<turnstile> P' { c } Q'"  |
-  inv[intro]:    "R,G \<turnstile> P {c} Q \<Longrightarrow> stable R' I \<Longrightarrow> G \<subseteq> R' \<Longrightarrow> R \<inter> R',G \<turnstile> (P \<inter> I) {c} (Q \<inter> I)" |
-  refine[intro]: "R,G \<turnstile> P {c} Q \<Longrightarrow> refine c c' \<Longrightarrow> R,G \<turnstile> P {c'} Q" |
-  aux[intro]:    "R,G \<turnstile> P {c} Q \<Longrightarrow> aux\<^sub>C r c c' \<Longrightarrow> aux\<^sub>R r R,aux\<^sub>G r G \<turnstile> aux\<^sub>P r P {c'} aux\<^sub>P r Q"
+                   R',G' \<turnstile> P' { c } Q'"  |
+  inv[intro]:    "R,G \<turnstile> P {c} Q \<Longrightarrow> stable R' I \<Longrightarrow> G \<subseteq> R' \<Longrightarrow> R \<inter> R',G \<turnstile> (P \<inter> I) {c} (Q \<inter> I)"
 
 subsection \<open>Properties\<close>
 
@@ -42,13 +35,7 @@ lemma nilE [elim!]:
   assumes "R,G \<turnstile> P {Nil} Q"
   obtains M where "stable R M" "P \<subseteq> M" "M \<subseteq> Q"
   using assms 
-proof (induct R G P "Nil :: ('a,'b) com" Q)
-  case (refine R G P c\<^sub>1 Q)
-  thus ?case by auto
-next
-  case (aux R G P c Q r)
-  thus ?case using aux\<^sub>P_mono aux_stable by blast
-qed blast+
+  by (induct R G P "Nil :: ('a,'b) com" Q) blast+
 
 lemma basicE [elim!]:
   assumes "R,G \<turnstile> P {Basic \<beta>} Q"
@@ -67,46 +54,22 @@ next
     case (1 P' Q')
     thus ?case using inv(3,4) inv(5)[of "P' \<inter> I" "Q' \<inter> I"] atomic_invI by blast
   qed
-next
-  case (refine R G P c Q)
-  then obtain \<alpha> where a: "c = Basic \<alpha>" "refine\<^sub>\<alpha> \<alpha> \<beta>" by (auto)
-  show ?case 
-  proof (rule refine(2)[OF a(1)], goal_cases)
-    case (1 P' Q')
-    then show ?case using refine(4) a(2) atomic_refineI by metis
-  qed
-next
-  case (aux R G P c Q r)
-  then obtain \<alpha> where a: "c = Basic \<alpha>" "aux\<^sub>\<alpha> r \<alpha> \<beta>" by (auto)
-  show ?case
-  proof (rule aux(2)[OF a(1)], goal_cases)
-    case (1 P' Q')
-    then show ?case using aux(4) a(2) atomic_auxI aux\<^sub>P_mono by metis
-  qed
 qed
 
 lemma seqE [elim]:
-  assumes "R,G \<turnstile> P {c\<^sub>1 ;; c\<^sub>2} Q"
+  assumes "R,G \<turnstile> P {c\<^sub>1 ; c\<^sub>2} Q"
   obtains M  where "R,G \<turnstile> P {c\<^sub>1} M" "R,G \<turnstile> M {c\<^sub>2} Q"
-  using assms 
-  by (induct R G P "c\<^sub>1 ;; c\<^sub>2" Q arbitrary: c\<^sub>1 c\<^sub>2) blast+ 
+  using assms by (induct R G P "c\<^sub>1 ; c\<^sub>2" Q arbitrary: c\<^sub>1 c\<^sub>2) blast+ 
 
-lemma ordE [elim]:
-  assumes "R,G \<turnstile> P {c\<^sub>1 \<cdot> c\<^sub>2} Q"
-  obtains M  where "R,G \<turnstile> P {c\<^sub>1} M" "R,G \<turnstile> M {c\<^sub>2} Q"
-  using assms by (induct R G P "c\<^sub>1 \<cdot> c\<^sub>2" Q arbitrary: c\<^sub>1 c\<^sub>2) blast+
 
 text \<open>It is always possible to rephrase a judgement in terms of a stable precondition\<close>
 lemma stable_preE:
   assumes "R,G \<turnstile> P {c} Q"
   shows "\<exists>P'. P \<subseteq> P' \<and> stable R P' \<and> R,G \<turnstile> P' {c} Q"
   using assms 
-proof (induct)
-  case (state R G P c Q op l)
-  then show ?case by (metis thr_stable thr_mono rules.state)
-next 
-  case (thread R G P c Q op)
-  then show ?case by (metis thr_stable' thr_mono' rules.thread)
+proof (induct) 
+  case (thread R G P c Q)
+  then show ?case by (metis rules.thread)
 next 
   case (par R\<^sub>1 G\<^sub>1 P\<^sub>1 c\<^sub>1 Q\<^sub>1 R\<^sub>2 G\<^sub>2 P\<^sub>2 c\<^sub>2 Q\<^sub>2)
   obtain P\<^sub>1' where 1: "P\<^sub>1 \<subseteq> P\<^sub>1'" "stable R\<^sub>1 P\<^sub>1'" "R\<^sub>1,G\<^sub>1 \<turnstile> P\<^sub>1' {c\<^sub>1} Q\<^sub>1" using par by auto
@@ -123,43 +86,13 @@ next
   have "stable R (P\<^sub>1 \<inter> P\<^sub>2)" using 1 2 by auto
   thus ?case using 1 2 by blast
 next
-  case (seqset S R G P Q)
-  hence "\<exists>P\<^sub>s. \<forall>s\<in>S. P \<subseteq> P\<^sub>s s \<and> stable R (P\<^sub>s s) \<and> (R,G \<turnstile> P\<^sub>s s {seq2com s} Q)"
-    by metis
-  then obtain P\<^sub>s where s: "\<forall>s\<in>S. P \<subseteq> P\<^sub>s s \<and> stable R (P\<^sub>s s) \<and> (R,G \<turnstile> P\<^sub>s s {seq2com s} Q)"
-    by blast
-  hence "stable R (\<Inter>s\<in>S. P\<^sub>s s)" by (auto simp: stable_def)
-  moreover have "P \<subseteq> (\<Inter>s\<in>S. P\<^sub>s s)" using s by auto
-  ultimately show ?case using s seqset.hyps(1) by blast
-next
   case (conseq R G P c Q P' R' G' Q')
   then show ?case by (meson order_refl rules.conseq stable_conseqI subset_trans)
 next
   case (inv R G P c Q R' I)
   then obtain P' where "P \<subseteq> P'" "stable R P'" "R,G \<turnstile> P' {c} Q" by auto
   then show ?case using inv rules.inv by blast
-next
-  case (aux R G P c Q r c')
-  thus ?case using aux\<^sub>P_mono aux_stable by (metis rules.aux)
 qed blast+
-
-lemma false_seqI [intro]:
-  "\<forall>\<beta> \<in> set s. guar\<^sub>\<alpha> \<beta> G \<Longrightarrow> R,G \<turnstile> {} {seq2com s} {}"
-  by (induct s) auto
-
-lemma falseI:
-  shows "local c \<Longrightarrow> \<forall>\<beta> \<in> basics c. guar\<^sub>\<alpha> \<beta> G \<Longrightarrow> UNIV,G \<turnstile> {} { c } {}"
-proof (induct c)
-  case (Basic x)
-  thus ?case by (intro basic) (auto simp: atomic_rule_def guar_def wp_def)
-next
-  case (SeqChoice x)
-  thus ?case by (intro ballI seqset false_seqI) auto
-qed auto
-
-lemma seq_rot:
-  "R,G \<turnstile> P { c\<^sub>1 } Q \<Longrightarrow> R,G \<turnstile> Q { c\<^sub>2 } M \<Longrightarrow> R,G \<turnstile> P { c\<^sub>1 ;; c\<^sub>2 } M" 
-  by auto
 
 end
 
