Semantics.thy
@@ -28,15 +28,14 @@ inductive lexecute :: "('a,'b) com \<Rightarrow> ('a,'b) com \<Rightarrow> ('a,'
   ("_ \<mapsto>[_,_] _" [71,0,0,71] 70)
   where
   act[intro]: "Basic \<alpha> \<mapsto>[Nil,\<alpha>] Nil" |
-  ino[intro]: "c\<^sub>1 \<mapsto>[r,\<alpha>] c\<^sub>1' \<Longrightarrow> c\<^sub>1 ;; c\<^sub>2 \<mapsto>[r,\<alpha>] c\<^sub>1' ;; c\<^sub>2" |
-  ord[intro]: "c\<^sub>1 \<mapsto>[r,\<alpha>] c\<^sub>1' \<Longrightarrow> c\<^sub>1 \<cdot> c\<^sub>2 \<mapsto>[r,\<alpha>] c\<^sub>1' \<cdot> c\<^sub>2" |
-  ooo[intro]: "c\<^sub>1 \<mapsto>[r,\<alpha>] c\<^sub>1' \<Longrightarrow> \<alpha>' < c\<^sub>2 ;; r <\<^sub>c \<alpha> \<Longrightarrow> c\<^sub>2 ;; c\<^sub>1 \<mapsto>[c\<^sub>2 ;; r ,\<alpha>] c\<^sub>2 ;; c\<^sub>1'"
+  ino[intro]: "c\<^sub>1 \<mapsto>[r,\<alpha>] c\<^sub>1' \<Longrightarrow> c\<^sub>1 ; c\<^sub>2 \<mapsto>[r,\<alpha>] c\<^sub>1' ; c\<^sub>2" |
+  ooo[intro]: "c\<^sub>1 \<mapsto>[r,\<alpha>] c\<^sub>1' \<Longrightarrow> \<alpha>' < c\<^sub>2 ; r <\<^sub>c \<alpha> \<Longrightarrow> c\<^sub>2 ; c\<^sub>1 \<mapsto>[c\<^sub>2 ; r ,\<alpha>] c\<^sub>2 ; c\<^sub>1'"
 inductive_cases lexecuteE[elim]: "c \<mapsto>[p,\<alpha>] c'"
 
 inductive gexecute :: "('a,'b) com \<Rightarrow> 'b rel \<Rightarrow> ('a,'b) com \<Rightarrow> bool"
   ("_ \<mapsto>[_] _" [71,0,71] 70)
   where
-  thr[intro]: "c \<mapsto>[r,\<alpha>] c' \<Longrightarrow> State l op c \<mapsto>[thr2glb op l l' (beh \<alpha>\<llangle>r\<rrangle>)] State l' op c'" |
+  thr[intro]: "c \<mapsto>[r,\<alpha>] c' \<Longrightarrow> Thread c \<mapsto>[beh \<alpha>\<llangle>r\<rrangle>] Thread c'" |
   par1[intro]: "c\<^sub>1 \<mapsto>[g] c\<^sub>1' \<Longrightarrow> c\<^sub>1 || c\<^sub>2 \<mapsto>[g] c\<^sub>1' || c\<^sub>2" |
   par2[intro]: "c\<^sub>2 \<mapsto>[g] c\<^sub>2' \<Longrightarrow> c\<^sub>1 || c\<^sub>2 \<mapsto>[g] c\<^sub>1 || c\<^sub>2'"
 inductive_cases gexecuteE[elim]: "c \<mapsto>[g] c'"
@@ -45,23 +44,20 @@ text \<open>Small step semantics for a silent step\<close>
 inductive silent :: "('a,'b) com \<Rightarrow> ('a,'b) com \<Rightarrow> bool"
   ("_ \<leadsto> _" [71,71] 70)
   where
-  seq1[intro]:  "c\<^sub>1 \<leadsto> c\<^sub>1' \<Longrightarrow> c\<^sub>1 ;; c\<^sub>2 \<leadsto> c\<^sub>1' ;; c\<^sub>2" |
-  ord1[intro]:  "c\<^sub>1 \<leadsto> c\<^sub>1' \<Longrightarrow> c\<^sub>1 \<cdot> c\<^sub>2 \<leadsto> c\<^sub>1' \<cdot> c\<^sub>2" |
-  seq2[intro]:  "c\<^sub>2 \<leadsto> c\<^sub>2' \<Longrightarrow> c\<^sub>1 ;; c\<^sub>2 \<leadsto> c\<^sub>1 ;; c\<^sub>2'" |
-  seqE1[intro]: "Nil ;; c\<^sub>1 \<leadsto> c\<^sub>1" |
-  seqE2[intro]: "c\<^sub>1 ;; Nil \<leadsto> c\<^sub>1" |
-  ordE[intro]:  "Nil \<cdot> c\<^sub>1 \<leadsto> c\<^sub>1" |
-  bigc[intro]:  "s \<in> S \<Longrightarrow> (\<Sqinter> S) \<leadsto> seq2com s" |
+  seq1[intro]:  "c\<^sub>1 \<leadsto> c\<^sub>1' \<Longrightarrow> c\<^sub>1 ; c\<^sub>2 \<leadsto> c\<^sub>1' ; c\<^sub>2" |
+  seq2[intro]:  "c\<^sub>2 \<leadsto> c\<^sub>2' \<Longrightarrow> c\<^sub>1 ; c\<^sub>2 \<leadsto> c\<^sub>1 ; c\<^sub>2'" |
+  seqE1[intro]: "Nil ; c\<^sub>1 \<leadsto> c\<^sub>1" |
+  seqE2[intro]: "c\<^sub>1 ; Nil \<leadsto> c\<^sub>1" |
   left[intro]:  "c\<^sub>1 \<sqinter> c\<^sub>2 \<leadsto> c\<^sub>1" |
   right[intro]: "c\<^sub>1 \<sqinter> c\<^sub>2 \<leadsto> c\<^sub>2" |
   loop1[intro]: "c* \<leadsto> Nil" |
-  loop2[intro]: "c* \<leadsto> c ;; c*" |
+  loop2[intro]: "c* \<leadsto> c ; c*" |
   par1[intro]:  "c\<^sub>1 \<leadsto> c\<^sub>1' \<Longrightarrow> c\<^sub>1 || c\<^sub>2 \<leadsto> c\<^sub>1' || c\<^sub>2" |
   par2[intro]:  "c\<^sub>2 \<leadsto> c\<^sub>2' \<Longrightarrow> c\<^sub>1 || c\<^sub>2 \<leadsto> c\<^sub>1 || c\<^sub>2'" |
   parE1[intro]: "Nil || c \<leadsto> c" |
   parE2[intro]: "c || Nil \<leadsto> c" |
-  stE[intro]:   "State l op Nil \<leadsto> Nil" |
-  thrE[intro]:  "Thread op c \<leadsto> State l op c"
+  thr[intro]:   "c \<leadsto> c' \<Longrightarrow> Thread c \<leadsto> Thread c'" |
+  thrE[intro]:  "Thread Nil \<leadsto> Nil"
 inductive_cases silentE[elim]: "c\<^sub>1 \<leadsto> c\<^sub>1'"
 
 text \<open>An execution step implies the program has changed\<close>
@@ -82,10 +78,6 @@ lemma gexecute_neq:
 lemma [simp]:
   "c \<mapsto>[g] c = False"
   using gexecute_neq by blast
-
-lemma [intro]:
-  "local (seq2com s)"
-  by (induct s) auto
 
 text \<open>A silent step will not introduce parallelism\<close>
 lemma local_silent:
