SimAsm_Rules.thy
@@ -1,0 +1,129 @@
+theory SimAsm_Rules
+  imports SimAsm
+begin
+
+section \<open>Wellformedness\<close>
+
+definition glb
+  where "glb m \<equiv> \<lambda>v. m (Glb v)"
+
+definition rg
+  where "rg m \<equiv> \<lambda>v. m (Reg v)"
+
+type_synonym ('v,'g) gstate = "'g \<Rightarrow> 'v"
+type_synonym ('v,'g) grel = "('v,'g) gstate rel"
+type_synonym ('v,'g,'r) trel = "('v,'g,'r) state rel"
+type_synonym ('v,'g,'r) trans = "('v,'g,'r) state set \<Rightarrow> ('v,'g,'r) state set"
+type_synonym ('v,'r,'a) rtrans = "('v,'r,'a) trel \<Rightarrow> ('v,'r,'a) trel"
+
+text \<open>Lift a relational predicate and assume it preserves the thread state\<close>
+definition step\<^sub>t :: "('v,'g) grel \<Rightarrow> ('v,'g,'r) trel"
+  where "step\<^sub>t R \<equiv> {(m,m'). (glb m, glb m') \<in> R \<and> rg m = rg m'}"
+
+text \<open>Define stability in terms of a relational predicate that preserves the thread state\<close>
+abbreviation stable\<^sub>t
+  where "stable\<^sub>t R P \<equiv> stable (step\<^sub>t R) P"
+
+definition stabilize
+  where "stabilize R P \<equiv> {m. \<forall>m'. (glb m,glb m') \<in> R \<longrightarrow> rg m = rg m' \<longrightarrow> m' \<in> P}"
+
+definition reflexive
+  where "reflexive R \<equiv> \<forall>m. (m,m) \<in> R"
+
+definition transitive
+  where "transitive R \<equiv> \<forall>m m' m''. (m,m') \<in> R \<longrightarrow> (m',m'') \<in> R \<longrightarrow> (m,m'') \<in> R"
+
+text \<open>Couple all wellformedness conditions into a single definition\<close>
+abbreviation wellformed :: "('v,'a) grel \<Rightarrow> ('v,'a) grel \<Rightarrow> bool"
+  where "wellformed R G \<equiv> reflexive R \<and> transitive R \<and> reflexive G" 
+
+text \<open>Show that a stabilized predicate is stable\<close>
+lemma stabilize_stable [intro]:
+  assumes wf: "wellformed R G"
+  shows "stable\<^sub>t R (stabilize R Q)"
+  unfolding stable_def step\<^sub>t_def
+proof (clarsimp)
+  fix m m'
+  assume a: "m \<in> stabilize R Q" "(glb m, glb m') \<in> R" "rg m = rg m'"
+  have "\<forall>g''. (glb m',g'') \<in> R \<longrightarrow> (glb m,g'') \<in> R"
+    using assms a(2) unfolding transitive_def by blast
+  thus "m' \<in> stabilize R Q" using a(1,3) by (auto simp: stabilize_def)
+qed
+
+text \<open>The conjunction of two stable predicates is stable\<close>
+lemma stable\<^sub>t_conj [intro]:
+  assumes "stable\<^sub>t R P" "stable\<^sub>t R Q"
+  shows "stable\<^sub>t R (P \<inter> Q)"
+  using assms by (auto simp: stable_def)
+
+text \<open>Elimination rule to ignore the stabilization process\<close>
+lemma stabilizeE:
+  assumes "m \<in> stabilize R P"
+  assumes "reflexive R"
+  obtains "m \<in> P"
+proof -
+  have "\<forall>g. (glb m, glb g) \<in> R \<longrightarrow> rg m = rg g \<longrightarrow> g \<in> P" "(glb m, glb m) \<in>  R"
+    using assms by (auto simp: reflexive_def stabilize_def)
+  thus ?thesis using that by auto
+qed
+
+text \<open>Stabilization preserves entailment\<close>
+lemma stabilize_entail [intro!]:
+  assumes "reflexive R"
+  assumes "P \<subseteq> Q"
+  shows "stabilize R P \<subseteq> Q"
+  using assms by (auto elim: stabilizeE)
+
+section \<open>Predicate Transformations\<close>
+
+named_theorems wp_defs
+
+text \<open>Transform a predicate based on an sub-operation\<close>
+fun wp\<^sub>i :: "('v,'g,'r) op \<Rightarrow> ('v,'g,'r) trans" 
+  where 
+    "wp\<^sub>i (assign r e) Q = {m. (m (r := ev m e)) \<in> Q}" |
+    "wp\<^sub>i (cmp b) Q =  {m. ev\<^sub>B m b \<longrightarrow> m \<in> Q}" | 
+    "wp\<^sub>i _ Q = Q"
+
+definition assert
+  where "assert b \<equiv> {m. b}"
+
+text \<open>Transform a predicate based on a program c within an environment R\<close>
+fun wp :: "('v,'g) grel \<Rightarrow> ('v,'g,'r) lang \<Rightarrow> ('v,'g,'r) trans"
+  where
+    "wp R Skip Q = Q" |
+    "wp R (Op v a) Q = stabilize R (v \<inter> wp\<^sub>i a Q)" |
+    "wp R (Seq c\<^sub>1 c\<^sub>2) Q = wp R c\<^sub>1 (wp R c\<^sub>2 Q)" |
+    "wp R (If b c\<^sub>1 c\<^sub>2) Q = (wp\<^sub>i (cmp b) (wp R c\<^sub>1 Q) \<inter> wp\<^sub>i (cmp (Neg b)) (wp R c\<^sub>2 Q))" |
+    "wp R (While b I c) Q = 
+      (stabilize R I \<inter> assert (I \<subseteq> wp\<^sub>i (cmp b) (wp R c (stabilize R I)) \<inter> wp\<^sub>i (cmp (Neg b)) Q))"
+
+text \<open>Convert a predicate transformer into a relational predicate transformer\<close>
+definition wp\<^sub>r :: "('v,'r,'a) trans \<Rightarrow> ('v,'r,'a) rtrans"
+  where "wp\<^sub>r f G \<equiv> {(m,m'). m' \<in> f {m'. (m,m') \<in> G}}"
+declare wp\<^sub>r_def [wp_defs]
+
+subsection \<open>Guarantee Checks\<close>
+
+text \<open>Convert a predicate transformer into a guarantee check\<close>
+abbreviation guar
+  where "guar f G \<equiv> {m. (m,m) \<in> (wp\<^sub>r f G)}"
+
+text \<open>Ensure all global operations in a thread conform to its guarantee\<close>
+fun guar\<^sub>c
+  where 
+    "guar\<^sub>c (Op v a) G = (v \<subseteq> guar (wp\<^sub>i a) G)" |
+    "guar\<^sub>c (Seq c\<^sub>1 c\<^sub>2) G = (guar\<^sub>c c\<^sub>1 G \<and> guar\<^sub>c c\<^sub>2 G)" |
+    "guar\<^sub>c (If _ c\<^sub>1 c\<^sub>2) G = (guar\<^sub>c c\<^sub>1 G \<and> guar\<^sub>c c\<^sub>2 G)" |
+    "guar\<^sub>c (While _ _ c) G = (guar\<^sub>c c G)" |
+    "guar\<^sub>c _ _ = False"
+
+text \<open>Correctness of the guarantee check\<close>
+lemma com_guar:
+  "wellformed R G \<Longrightarrow> guar\<^sub>c c G \<Longrightarrow> \<forall>\<beta>\<in>basics c. guar\<^sub>\<alpha> \<beta> G"
+proof (induct c)
+  case (Basic x)
+  then show ?case apply (cases "tag x") apply (auto simp: guar_def wp\<^sub>r_def) sorry
+qed auto
+
+end
